revert, use many

src/ExampleParser.v
@@ -37,9 +37,11 @@ Class Biparser (P : Type -> Type -> Type) :=
   { Biparser_Profmonad :> Profmonad P;
     Biparser_Partial :> forall U, MonadPartial (P U);
     biparse_token : P t t;
+    biparse_many : forall U A, P (option U) (option A) -> P (list U) (list A)
   }.
 
 Arguments biparse_token {P _}.
+Arguments biparse_many {P _  U A}.
 
 (** ** Example biparsers *)
 
@@ -85,7 +87,8 @@ Definition biparse_string `{Biparser P} : P (list nat) (list nat) :=
 #[global]
 Instance Biparser_product P1 P2 `{Biparser P1, Biparser P2} :
   Biparser (Product P1 P2) :=
-  { biparse_token := (biparse_token, biparse_token);
+  { biparse_token := (biparse_token, biparse_token)
+  ; biparse_many := fun U A p => (biparse_many (fst p), biparse_many (snd p))
   }.
 
 (** *** Parser promonad ***)
@@ -93,15 +96,40 @@ Instance Biparser_product P1 P2 `{Biparser P1, Biparser P2} :
 (** Input streams *)
 Definition stream := list t.
 
+Module Delay.
+
+CoInductive m (A : Type) : Type := Wait { step : m A + A }.
+
+Arguments Wait {A}.
+Arguments step {A}.
+
+Definition flip_bind {A B} (k : A -> m B) : m A -> m B := cofix bind_ u :=
+  Wait match step u with
+  | inl more => inl (bind_ more)
+  | inr x => step (k x)
+  end.
+
+#[global] Instance Monad_delay : Monad m :=
+  {| ret := fun _ x => Wait (inr x)
+  ;  bind := fun _ _ u k => flip_bind k u
+  |}.
+
+End Delay.
+
+Notation delay := Delay.m.
+
 (** **** Parser monad *)
 
-Definition parser (A : Type) : Type := stream -> option (A * stream).
+Definition parser (A : Type) : Type := stream -> delay (option (A * stream)).
 
 #[global]
 Instance Monad_parser : Monad parser :=
-  { ret A x := fun s => Some (x, s);
+  { ret A x := fun s => ret (Some (x, s));
     bind A B m k := fun s =>
-      bind (m s) (fun '(a, s') => k a s')
+      bind (m s) (fun xs => match xs with
+      | None => ret None
+      | Some (a, s') => k a s'
+      end)
   }.
 
 #[global]
@@ -137,6 +165,9 @@ Instance MonadPartial_parser : MonadPartial parser :=
 Definition parser2 := Fwd parser.
 
 Definition Profmonad_parser2 := Profmonad_Fwd parser.
+
+Definition parse_many {A} (u : parser (option A)) : parser (list A) :=
+  match
 
 #[global]
 Instance Biparser_parser2 : Biparser parser2 :=
@@ -270,34 +301,26 @@ Definition right_round_trip A (pa : parser2 A A) (pr : printer2 A A)
     | Some _ => True
     end.
 
-Definition backward {A} (P : A -> Prop) (p : biparser A A) : Prop :=
-  forall (a : A),
-    P a ->
-    exists s,
-    (exists a', snd p a = Some (s, a')) /\
-    (forall s', fst p (s ++ s') = Some (a, s')).
+Definition backward {A} (p : biparser A A) : Prop :=
+  forall (a : A) (s s' : list t),
+    (exists a', snd p a = Some (s, a')) ->
+    fst p (s ++ s') = Some (a, s').
 
-Definition forward {A} (P : A -> Prop) (p : biparser A A) : Prop :=
-  forall (a : A) (s01 s1 : list t),
+Definition forward {A} (p : biparser A A) : Prop :=
+  forall (a : A) (s01 s1 s0 : list t),
     fst p s01 = Some (a, s1) ->
-    forall s0,
-    ((exists a', snd p a = Some (s0, a')) ->
-    s01 = s0 ++ s1).
+    (exists a', snd p a = Some (s0, a')) ->
+    s01 = s0 ++ s1.
 
 (** *** Weak but compositional roundtrip properties *)
 
-Definition weak_backward {U A} (P : U -> Prop) (p : biparser U A) : Prop :=
+Definition weak_backward {U A} (p : biparser U A) : Prop :=
   forall (u : U) (a : A) (s s' : list t),
-    P u ->
     snd p u = Some (s, a) ->
     fst p (s ++ s') = Some (a, s').
 
-Definition satisfies {U A} (P : A -> Prop) (p : biparser U A) : Prop :=
-  (forall (a : A) s01 s1, fst p s01 = Some (a, s1) -> P a) /\
-  (forall (a : A) (u : U) s0, snd p u = Some (s0, a) -> P a).
-
 Definition weak_forward {U A} (p : biparser U A) : Prop :=
-  forall (a : A) (u : U) (s01 s0 s1 : list t),
+  forall (u : U) (a : A) (s01 s1 s0 : list t),
     fst p s01 = Some (a, s1) ->
     snd p u = Some (s0, a) ->
     s01 = s0 ++ s1.
@@ -307,109 +330,97 @@ Definition weak_forward {U A} (p : biparser U A) : Prop :=
 Definition purify {U V} (p : biparser U V) : pfunction U V :=
   fun a => option_map snd (snd p a).
 
-Definition aligned {A} (P : A -> Prop) (p : biparser A A) : Prop :=
-  forall (a : A), P a -> purify p a = Some a.
+Definition aligned {A} (p : biparser A A) : Prop :=
+  forall (a : A),
+    exists s0, snd p a = Some (s0, a).
 
-Definition aligned_ {U A} (P : U -> Prop) (f : U -> A) (p : biparser U A) : Prop :=
-  forall (u : U), P u -> purify p u = Some (f u).
+Definition aligned_ {U A} (f : U -> A) (p : biparser U A) : Prop :=
+  forall (u : U),
+    (exists s0, snd p u = Some (s0, f u)).
+
+Definition aligned' {A} (p : pfunction A A) : Prop :=
+  forall (a : A), p a = Some a.
+
+Theorem aligned_equiv {A} (p : biparser A A)
+  : aligned p <-> aligned' (purify p).
+Proof.
+  split; intros H a; unfold aligned, aligned', purify in *.
+  - destruct (H a) as [s E].
+    rewrite E; reflexivity.
+  - specialize (H a).
+    destruct (snd p a) as [ [] | ]; cbn in H; try discriminate.
+    injection H; intros []; eauto.
+Qed.
 
 (** ** Connection between strong and weak roundtrip properties **)
 
-Theorem backward_aligned {A} (P : A -> Prop) (p : biparser A A) :
-  aligned P p ->
-  weak_backward P p ->
-  backward P p.
+Theorem backward_aligned {A} (p : biparser A A) :
+  aligned p ->
+  weak_backward p ->
+  backward p.
 Proof.
-  intros ALIGNED WBWD a Pa.
-  specialize (ALIGNED a Pa).
-  unfold purify in ALIGNED.
-  destruct (snd p a) as [[s a']|] eqn:Esnd; inversion ALIGNED; subst.
-  exists s.
-  split; [ eauto | ].
-  intros s'.
-  eapply WBWD; eauto.
+  intros ALIGNED WBWD a s s' [a' Ea].
+  destruct (ALIGNED a).
+  rewrite Ea in H.
+  injection H; intros [] [].
+  apply (WBWD _ _ _ _ Ea).
 Qed.
 
-Theorem forward_aligned {A} (P : A -> Prop) (p : biparser A A) :
-  satisfies P p ->
-  aligned P p ->
+Theorem forward_aligned {A} (p : biparser A A) :
+  aligned p ->
   weak_forward p ->
-  forward P p.
+  forward p.
 Proof.
-  intros SAT ALIGNED WFWD a s01 s1 E01 s0 [a' H3].
-  assert (Pa := proj1 SAT a _ _ E01).
-  specialize (ALIGNED a Pa).
-  unfold purify in ALIGNED.
-  rewrite H3 in ALIGNED; inversion ALIGNED; clear ALIGNED; subst.
-  apply (WFWD a a _ _ _ E01 H3).
+  intros ALIGNED WFWD a s01 s1 s0 E01 [a' E0].
+  destruct (ALIGNED a).
+  rewrite E0 in H.
+  injection H. intros; subst.
+  eapply WFWD; eauto.
 Qed.
 
 (** ** Compositionality of weak roundtrip properties *)
 
-Lemma weak_backward_ret U A (P : U -> Prop) (a : A) : weak_backward P (ret a).
+Lemma weak_backward_ret U A (a : A) : @weak_backward U A (ret a).
 Proof.
-  intros u b s s' Pu e; inversion_clear e; reflexivity.
+  intros u b s s' e; inversion_clear e; reflexivity.
 Qed.
 
-Definition comapProp {U U'} (f : U -> option U') (P : U -> Prop) (u' : U') : Prop :=
-  exists u, f u = Some u' /\ P u.
-
-Lemma weak_backward_comap U U' A (P : U -> Prop) (f : U -> option U')
+Lemma weak_backward_comap U U' A (f : U -> option U')
       (m : biparser U' A)
-      (Hm : weak_backward (comapProp f P) m) :
-  weak_backward P (comap f m).
+      (Hm : weak_backward m) :
+  weak_backward (comap f m).
 Proof.
-  intros u b s s' Pu e.
+  intros u b s s' e.
   cbn in *.
   destruct (f u) eqn:ef; try discriminate.
   destruct snd as [[] | ] eqn:E.
   - cbn in e. rewrite app_nil_r in e. injection e. intros ? ?; subst. clear e.
     eapply Hm in E.
-    + rewrite E; eauto.
-    + red. exists u; auto.
+    rewrite E.
+    eauto.
   - discriminate.
 Qed.
 
-Lemma weak_backward_bind U A B (P : U -> Prop)
+Lemma weak_backward_bind U A B
       (m : biparser U A) (k : A -> biparser U B)
-      (Hm : weak_backward P m)
-      (Hk : forall a, weak_backward P (k a)) :
-  weak_backward P (bind m k).
+      (Hm : weak_backward m)
+      (Hk : forall a, weak_backward (k a)) :
+  weak_backward (bind m k).
 Proof.
-  intros u b s s' Pu.
-  cbn in *.
+  intros u b s s'.
+  simpl.
   destruct (snd m u) as [ [s1 a] | ] eqn:em; simpl; try discriminate.
   destruct (snd (k a) u) as [ [s2 b'] | ] eqn:ek; simpl; try discriminate.
   intros Hmk.
   inversion Hmk.
-  eapply (Hm _ _ _ _ Pu) in em.
-  eapply (Hk _ _ _ _ _ Pu) in ek.
+  eapply Hm in em.
+  eapply Hk in ek.
   rewrite <- app_assoc.
   rewrite em; simpl.
   rewrite ek.
   subst; reflexivity.
 Qed.
 
-Class Compositional
-      {P : Type -> Type -> Type}
-      `{Profmonad P}
-      (R : forall A B, (A -> Prop) -> P A B -> Prop) : Prop :=
-  {
-    CompositionalWithLawful :> ProfmonadLaws _;
-    ret_comp :
-      forall U A (F : U -> Prop) (a : A), R U A F (ret a : P U A);
-    bind_comp :
-      forall U A B (F : U -> Prop) (m : P U A) (k : A -> P U B) ,
-        R U A F m ->
-        (forall a, R U B F (k a)) ->
-        R U B F (bind m k);
-    comap_comp :
-      forall U V A (F : U -> Prop) (f : U -> option V) (m : P V A),
-        R V A (comapProp f F) m ->
-        R U A F (comap f m);
-  }.
-
-#[global]
 Instance Compositional_weak_backward :
   Compositional (@weak_backward) := {
   ret_comp := weak_backward_ret;
@@ -417,45 +428,48 @@ Instance Compositional_weak_backward :
   comap_comp := weak_backward_comap;
 }.
 
-Lemma weak_backward_empty U A P :
-  weak_backward P (@empty (biparser U) _ _ A).
+Lemma weak_backward_empty U A :
+  weak_backward (@empty (biparser U) _ _ A).
 Proof.
   discriminate.
 Qed.
 
-Lemma weak_backward_token P :
-  weak_backward P biparse_token.
+Lemma weak_backward_token :
+  weak_backward biparse_token.
 Proof.
-  intros u b s s' Pu H; inversion H; subst; reflexivity.
+  intros u b s s' H; inversion H; subst; reflexivity.
 Qed.
 
 Lemma weak_forward_ret U A (a : A) : @weak_forward U A (ret a).
 Proof.
-  intros a' b s01 s0 s1 e1 e2; inv e1; inv e2; reflexivity.
+  intros u b s s' s'' e e';
+    inversion_clear e; inversion_clear e'; reflexivity.
 Qed.
 
 Lemma weak_forward_comap U U' A (f : U -> option U')
-      (m : biparser U' A) (Hm : weak_forward m) :
+      (m : biparser U' A)
+      (Hm : weak_forward m) :
   weak_forward (comap f m).
 Proof.
-  intros a u s01 s0 s1 e1 e2.
+  intros u b s s' s'' e e'.
   cbn in *.
-  destruct (fst m) as [[]|] eqn:E1; cbn in e1; inv e1.
   destruct (f u) eqn:ef; try discriminate.
-  destruct (snd m) as [[]|] eqn:E2; cbn; inv e2.
+  destruct fst as [[]|] eqn:E1; try discriminate.
+  destruct snd as [[]|] eqn:E2; try discriminate.
+  cbn in *.
+  injection e; injection e'; intros; subst; clear e e'.
   rewrite app_nil_r.
-  eapply Hm; eauto.
+  eapply Hm; eassumption.
 Qed.
 
-Lemma weak_forward_bind U A B (P : A -> Prop)
+Lemma weak_forward_bind U A B
       (m : biparser U A) (k : A -> biparser U B) (f : B -> option A)
-      (Sm : satisfies P m)
+      (Hf : forall a, (x <- k a;; ret (f x)) = (x <- k a;; ret (Some a)))
       (Hm : weak_forward m)
-      (Hf : forall a, P a -> (x <- k a;; ret (f x)) = (x <- k a;; ret (Some a)))
-      (Hk : forall a, P a -> weak_forward (k a)) :
+      (Hk : forall a, weak_forward (k a)) :
   weak_forward (bind m k).
 Proof.
-  intros b u s01 s0 s1 Hparse Hprint.
+  intros u b s01 s1 s0 Hparse Hprint.
   simpl in *.
   destruct fst as [ [a1 s__m1] | ] eqn:em1 in Hparse; try discriminate;
     simpl in Hparse;
@@ -465,147 +479,40 @@ Proof.
     simpl in Hprint;
     destruct snd as [ [s__mk2 b2] | ] eqn:ek2 in Hprint; try discriminate;
     inversion Hprint; clear Hprint; subst.
-  assert (Pa1 : P a1). { apply (proj1 Sm _ _ _ em1). }
-  assert (Pa2 : P a2). { apply (proj2 Sm _ _ _ em2). }
-  assert (ea : a2 = a1); [ | subst a2 ].
-  { pose proof (Hf a1 Pa1) as Hf1.
-    apply (f_equal (fun f => fst f s__m1)) in Hf1. simpl in Hf1.
+  assert (ea : a2 = a1).
+  { pose proof (Hf a1) as Hf1.
+    apply (f_equal (fun f => fst f s__m1)) in Hf1; simpl in Hf1.
     rewrite ek1 in Hf1; inversion Hf1.
-    pose proof (Hf a2 Pa2) as Hf2.
+    pose proof (Hf a2) as Hf2.
     apply (f_equal (fun f => snd f u)) in Hf2; simpl in Hf2.
     rewrite ek2 in Hf2; inversion Hf2.
     rewrite H0 in H1; inversion H1.
     reflexivity.
   }
-  specialize (Hm _ _ _ _ _ em1 em2).
-  specialize (Hk _ Pa1 _ _ _ _ _ ek1 ek2).
-  rewrite <- app_assoc, <- Hk, <- Hm. reflexivity.
+  subst.
+  specialize (Hm u a1 s01 s__m1 s__m2 em1 em2).
+  specialize (Hk a1 u b s__m1 s1 s__mk2 ek1 ek2).
+  subst.
+  apply app_assoc.
 Qed.
 
-Class WP (P : Type -> Type -> Type) `{Profmonad P} (S : forall A B, (B -> Prop) -> P A B -> Prop)
-  : Prop :=
-  { ret_wp : forall U A a, S U A (eq a) (ret a);
-    bind_wp : forall U A B (F G : _ -> Prop) (m : P U A) (k : A -> P U B),
-      S U A F m -> (forall a, F a -> S U B G (k a)) -> S U B G (bind m k);
-    comap_wp : forall U V A (F : _ -> Prop) (f : U -> option V) (m : P V A),
-      S V A F m -> S U A F (comap f m);
-    mono_wp : forall U A (F G : A -> Prop) (m : P U A),
-      (forall a, F a -> G a) ->
-      S U A F m -> S U A G m
-  }.
-
-Class Quasicompositional'
-      (P : Type -> Type -> Type)
-      `{Profmonad P}
-      (S : forall A B, (B -> Prop) -> P A B -> Prop)
-      `{WP P S}
-      (R : forall A B, P A B -> Prop) : Prop :=
-  {
-    ret_comp' :
-      forall A0 A a, R A0 A (ret a);
-    bind_comp' :
-      forall U A B (F : _ -> Prop) (m : P U A) (k : A -> P U B) (f : B -> option A),
-        S U A F m ->
-        R U A m ->
-        (forall a, F a -> (x <- k a;; ret (f x)) = (x <- k a;; ret (Some a))) ->
-        (forall a, F a -> R U B (k a)) ->
-        R U B (bind m k);
-    comap_comp' :
-      forall U V A (f : U -> option V) (m : P V A),
-        R V A m -> R U A (comap f m)
-  }.
-
-Class Quasicompositional (P : Type -> Type -> Type) `{Profmonad P} (R : forall {A B}, (B -> Prop) -> P A B -> Prop) : Prop :=
-  { ret_qcomp : forall U A a, @R U A (eq a) (ret a)
-  ; bind_qcomp : forall U A B (F G : _ -> Prop) (m : P U A) (k : A -> P U B) (f : B -> option A),
-      R F m ->
-      (forall a, F a -> (x <- k a;; ret (f x)) = (x <- k a;; ret (Some a))) ->
-      (forall a, F a -> R G (k a)) ->
-      R G (bind m k)
-  ; comap_qcomp : forall U V A F (f : U -> option V) (m : P V A),
-      R F m -> R F (comap f m)
-  ; mono_qcomp : forall U A (F G : A -> Prop) (m : P U A),
-      (forall a, F a -> G a) -> R F m -> R G m
-  }.
-
-Definition wp_roundtrip {P : Type -> Type -> Type} (S : forall A B, (B -> Prop) -> P A B -> Prop) (R : forall A B, P A B -> Prop) : forall A B, (B -> Prop) -> P A B -> Prop :=
-  fun A B F m => S A B F m /\ R A B m.
-
-Lemma Quasi {P : Type -> Type -> Type} `{Profmonad P} S `{HS : WP P S} R
-  : Quasicompositional' P S R -> Quasicompositional P (wp_roundtrip S R).
-Proof.
-  intros QC; constructor.
-  - constructor; [ apply HS | apply QC ].
-  - intros * Hm Hinj Hk. constructor; [ eapply bind_wp; [apply Hm | apply Hk] | eapply bind_comp'; [apply Hm| apply Hm | apply Hinj | apply Hk] ].
-  - intros * Hm. constructor; [ apply comap_wp | apply comap_comp' ]; apply Hm.
-  - intros * HF Hm; split; [ eapply mono_wp |]; [ apply HF | apply Hm .. ].
-Qed.
-
-Lemma bind_comap_comp' {P} {R : forall A B, (B -> Prop) -> P A B -> Prop}
-    `{Quasicompositional P R}
-  : forall A B (F G : _ -> Prop) (m : P A A) (k : A -> P B B) (f : B -> option A),
-      (forall a, F a -> (x <- k a;; ret (f x)) = (x <- k a;; ret (Some a))) ->
-      R A A F m ->
-      (forall a, F a -> R B B G (k a)) ->
-      R B B G (bind (comap f m) k).
-Proof.
-  intros. eapply (bind_qcomp _ _ _ _ _ _ _ f); eauto.
-  apply comap_qcomp; eauto.
-Qed.
-
-Definition weak_forward' {A B} := wp_roundtrip (@satisfies) (@weak_forward) A B.
-
-Section A.
-#[local]
-Instance WP_satisfies : WP biparser (@satisfies).
-Proof.
-  constructor.
-  - split; intros * Hret; inv Hret; auto.
-  - intros * Hm Hk; split; intros *; cbn.
-    + destruct (fst m) as [[a' s]|] eqn:Em1; cbn; try discriminate.
-      intros Ek1.
-      apply Hm in Em1.
-      apply (proj1 (Hk _ Em1) _ _ _ Ek1).
-    + destruct (snd m) as [[s  a'] | ] eqn:Em2; cbn; try discriminate.
-      destruct (snd (k _)) as [[s' b'] | ] eqn:Ek2; cbn; try discriminate.
-      intros HH; inv HH.
-      apply Hm in Em2.
-      apply (proj2 (Hk _ Em2) _ _ _ Ek2).
-  - intros * Hm; split; intros *; cbn.
-    + destruct (fst m) as [[a' s]|] eqn:Em1; cbn; try discriminate.
-      intros HH; inv HH.
-      eapply (proj1 Hm); eauto.
-    + destruct (f u); cbn; try discriminate.
-      destruct (snd m) as [[s b]|] eqn:Em2; cbn; try discriminate.
-      intros HH; inv HH.
-      eapply (proj2 Hm); eauto.
-  - intros * HF []; split; eauto.
-Qed.
-
-#[global]
 Instance Quasicompositional_weak_forward :
-  Quasicompositional' biparser (@satisfies) (@weak_forward) := {
+  Quasicompositional (@weak_forward) := {
   ret_comp' := weak_forward_ret;
   bind_comp' := weak_forward_bind;
   comap_comp' := weak_forward_comap;
 }.
 
-Lemma weak_forward_empty_ U A : weak_forward (@empty (biparser U) _ _ A).
-Proof. discriminate. Qed.
-
-Lemma satisfies_empty U A : satisfies (fun _ => False) (@empty (biparser U) _ _ A).
-Proof. split; discriminate. Qed.
-
 Lemma weak_forward_empty U A :
-  weak_forward' (fun _ => False) (@empty (biparser U) _ _ A).
+  weak_forward (@empty (biparser U) _ _ A).
 Proof.
-  split; [ apply satisfies_empty | apply weak_forward_empty_ ].
+  discriminate.
 Qed.
 
 Lemma weak_forward_token :
-  weak_forward (fun _ => True) biparse_token.
+  weak_forward biparse_token.
 Proof.
-  intros b s s' H1. split; [auto | intros u s0 H2].
+  intros u b s s' s'' H1 H2.
   destruct s; simpl in *.
   - discriminate.
   - inversion H1; inversion H2; subst.
@@ -614,18 +521,18 @@ Qed.
 
 (**)
 
-Lemma weak_forward_digit {b} : weak_forward (fun _ => True) (biparse_digit b).
+Lemma weak_forward_digit {b} : weak_forward (biparse_digit b).
 Proof.
   unfold biparse_digit; intros.
-  eapply bind_comap_comp'.
+  apply bind_comap_comp'.
   { intros a; destruct lt_dec; cbn; reflexivity. }
   { apply weak_forward_token. }
   { intros a; destruct lt_dec.
-    - eapply weaken_weak_forward, weak_forward_ret; constructor.
-    - eapply weaken_weak_forward, weak_forward_empty; constructor. }
+    - apply weak_forward_ret.
+    - apply weak_forward_empty. }
 Qed.
 
-Lemma weak_backward_digit {b} P : weak_backward P (biparse_digit b).
+Lemma weak_backward_digit {b} : weak_backward (biparse_digit b).
 Proof.
   unfold biparse_digit.
   apply bind_comp.
@@ -636,53 +543,18 @@ Proof.
     + apply weak_backward_empty.
 Qed.
 
-Lemma strengthen_weak_backward {U A} (P Q : _ -> Prop) (p : biparser U A)
-  : (forall u, P u -> Q u) ->
-    weak_backward Q p -> weak_backward P p.
+Lemma weak_backward_replicate {A} {n} {p : biparser A A}
+  : weak_backward p ->
+    weak_backward (replicate n p).
 Proof.
-  unfold weak_backward. eauto.
+  apply replicate_comp; typeclasses eauto.
 Qed.
 
-Lemma weak_backward_replicate {A} {n} {p : biparser A A} (P Q : _ -> Prop)
-  : (forall xs, Q xs -> length xs = n /\ Forall P xs) ->
-    weak_backward P p ->
-    weak_backward Q (replicate n p).
+Lemma weak_forward_replicate {A} {n} {p : biparser A A}
+  : weak_forward p ->
+    weak_forward (replicate n p).
 Proof.
-  intros F Hp.
-  revert Q F; induction n; cbn [replicate]; intros.
-  - apply weak_backward_ret.
-  - apply bind_comp.
-    { apply comap_comp.
-      eapply strengthen_weak_backward; [ | apply Hp ].
-      intros u [? [? ?]].
-      destruct x; inv H.
-      apply F in H0.
-      apply (Forall_inv (proj2 H0)). }
-    intros. apply bind_comp.
-    { apply comap_comp.
-      apply IHn.
-      intros xs [? [? ?]]. destruct x; inv H.
-      apply F in H0.
-      destruct H0.
-      inv H. inv H0. split; auto. }
-    intros; apply weak_backward_ret.
-Qed.
-
-Lemma weak_forward_replicate {A} (P : A -> Prop) (Q : list A -> Prop)  {n} {p : biparser A A}
-  : (forall xs, length xs = n /\ Forall P xs -> Q xs) ->
-    weak_forward P p ->
-    weak_forward Q (replicate n p).
-Proof.
-  intros F Hp.
-  revert Q F; induction n; cbn [replicate]; intros.
-  - apply (weaken_weak_forward (eq [])); [ | apply weak_forward_ret ].
-    intros _ <-; apply (F []); auto.
-  - eapply bind_comap_comp'; [ | eassumption | ].
-    { intros; rewrite 2 bind_bind; reflexivity. }
-    intros a.
-    eapply bind_comap_comp'; [ | | ].
-    { reflexivity. }
-    { eapply IHn. intros xs [<- all].
+  apply replicate_comp; typeclasses eauto.
 Qed.
 
 Lemma digit_unique {b} (d1 d2 : digit b) : proj1_sig d1 = proj1_sig d2 -> d1 = d2.
@@ -764,28 +636,3 @@ Proof.
   2:{ intros a; apply weak_forward_replicate. apply weak_forward_token. }
   { apply replicate_length_. }
 Qed.
-
-Lemma purify_bind {U A B} (p : biparser U A) (k : A -> biparser U B)
-  : forall u, purify (bind p k) u = bind (purify p u) (fun a => purify (k a) u).
-Proof.
-  intros u.
-  unfold purify; cbn.
-  destruct (snd p u) as [[] | ]; cbn; [ | reflexivity ].
-  destruct (snd (k a) u) as [[] | ]; cbn; reflexivity.
-Qed.
-
-Lemma purify_comap {U V A} (p : biparser V A) (f : U -> option V)
-  : forall u, purify (comap f p) u = bind (f u) (purify p).
-Proof.
-  intros u; unfold purify; cbn.
-  destruct (f u); cbn; [ | reflexivity ].
-  destruct (snd p v) as [[] |]; cbn; reflexivity.
-Qed.
-
-Theorem aligned_string : aligned biparse_string.
-Proof.
-  intros s.
-  unfold biparse_string.
-  rewrite purify_bind.
-  rewrite purify_comap.
-  cbn [bind Monad_option bind_option].
